# 1B2
## FysAB2
### 6.1
#### d.
$$p_f=\frac{h}{\lambda}$$

---
$$f=\frac{c}{\lambda}$$
$$\lambda=\frac{c}{f}$$
$$p_f=\frac{h\cdot (\frac{c}{6,56\cdot10^{-7}m}\cdot 2)}{c}=2,02\cdot10^{-27}Jm/s$$
## Kv6 Comtoneffekt
### 1.
$$\Updelta\lambda=\frac{h}{m_e\cdot c}(1-\cos\theta)$$

$$\frac{\lambda}{\lambda_c}=1-\cos\theta$$
$$-\frac{\lambda}{\lambda_c}+1=\cos\theta$$
$$\theta=\cos^{-1}\left(1-\frac{\lambda}{\lambda_c}\right)$$
$$\theta=\cos^{-1}\left(1-\frac{3,5\cdot10^{-12}}{\lambda_c}\right)=116,264\degree$$
### 2.
$$\Updelta\lambda=\lambda_c(1-\cos\theta)$$
$$E_f=h\cdot f$$
$$f=\frac{c}{\lambda}$$
$$\lambda=\frac{c}{f}$$
---

$$E=h\cdot f_1 - h\cdot f_2$$
$$E=h\cdot10^{19}Hz-h\cdot0,99\cdot10^{19}Hz=6,626\cdot10^{-17}J$$

### 3. $\theta=150\degree \lambda=10^{-12}m \lambda'=?$
#### a)
$$\Updelta\lambda=\lambda'-\lambda=\lambda_c(1-\cos\theta)$$
$$\lambda'-\lambda=\lambda_c(1-\cos\theta)$$
$$\lambda'=\lambda_c(1-\cos\theta)+\lambda$$
$$\lambda'=\lambda_c(1-\cos(150\degree))+10^{-12}m=5,528\cdot10^{-12}m$$
#### b)
$$E_f=h\cdot \frac{c}{(\lambda_c(1-\cos(150\degree))+10^{-12}m)-10^{-12}m}$$


